Revert "Phase 8: Lambda/SCall minimal model (Rocq + Lean)"
This reverts commit fdb4c8d7ac33d169d7f15691fe499cf34f4db5de.

src/formal-semantics/rocq/extracted/EmitExtract.ml
@@ -211,11 +211,6 @@ type contract_expr =
 | CGMake of contract_expr * contract_expr
 | CGCopy of ident
 | CGCopyRange of ident * contract_expr * contract_expr
-| CValid of contract_expr * contract_expr
-| CSeparated of contract_expr * contract_expr
-| CLength2d of ident
-| CValid2d of contract_expr * contract_expr * contract_expr
-| CClassInvariant of ident * contract_expr
 
 type aug_op =
 | AugAdd
@@ -258,9 +253,6 @@ type stmt =
 | SFieldAugAssign of ident * ident * binop * expr
 | SCritical of ident * stmt
 | SThreadEntry of stmt
-| SAcquires of ident
-| SReleases of ident
-| SCall of ident * expr * expr
 
 type whyml_exc =
 | ExcReturn
